src/SDK/Keyring/Defs.dfy
@@ -10,8 +10,8 @@ module {:extern "KeyringDefs"} KeyringDefs {
   import AlgorithmSuite
 
   trait {:termination false} Keyring {
-    ghost const Repr : set<object>
-    predicate Valid()
+    ghost var Repr : set<object>
+    predicate Valid() reads this, Repr
 
     method OnEncrypt(materials: Materials.ValidEncryptionMaterials) returns (res: Result<Materials.ValidEncryptionMaterials>)
       requires Valid()
@@ -23,8 +23,6 @@ module {:extern "KeyringDefs"} KeyringDefs {
           && materials.keyringTrace <= res.value.keyringTrace
           && materials.encryptedDataKeys <= res.value.encryptedDataKeys
           && materials.signingKey == res.value.signingKey
-      // TODO-RS: Temporary to let everything compile, hoping to not have to do this permanently.
-      decreases *
 
     method OnDecrypt(materials: Materials.ValidDecryptionMaterials,
                      encryptedDataKeys: seq<Materials.EncryptedDataKey>) returns (res: Result<Materials.ValidDecryptionMaterials>)
@@ -38,9 +36,5 @@ module {:extern "KeyringDefs"} KeyringDefs {
           && (materials.plaintextDataKey.Some? ==> res.value.plaintextDataKey == materials.plaintextDataKey)
           && materials.keyringTrace <= res.value.keyringTrace
           && res.value.verificationKey == materials.verificationKey
-      // TODO-RS: Temporary to let everything compile, hoping to not have to do this permanently.
-      decreases *
   }
- 
-  type ValidKeyring? = k: Keyring? | k == null || k.Valid()
 }
