src/SDK/Keyring/RawRSAKeyring.dfy
@@ -26,6 +26,7 @@ module {:extern "RawRSAKeyringDef"} RawRSAKeyringDef {
     const privateKey: Option<RSA.PrivateKey>
 
     predicate Valid()
+      reads this, Repr
     {
       this in Repr &&
       (publicKey.Some? || privateKey.Some?) &&
